PktClass.v
@@ -1,0 +1,78 @@
+From MyProject Require Import CrTransformer.
+From MyProject Require Import CrDsl.
+From MyProject Require Import Integers.
+From MyProject Require Import MyInts.
+From MyProject Require Import Maps.
+From MyProject Require Import CrIdentifiers.
+From MyProject Require Import CrVal.
+From MyProject Require Import CrProgramState.
+From MyProject Require Import CrVarLike.
+From MyProject Require Import CrConcreteSemanticsTransformer.
+
+From Stdlib Require Import ZArith.
+From Stdlib Require Import List.
+Import ListNotations.
+
+Definition Class := uint8. (* TODO: there's probably a better rep. *)
+Definition FilterDatabase := list (MatchPattern * Class).
+
+Definition PacketHeader := PMap.t CrVal.
+Definition Classifier :=
+  FilterDatabase -> PacketHeader -> option Class.
+
+Definition Interpretation := ConcreteState -> option Class.
+
+Fixpoint db_to_simple_helper (f : FilterDatabase) (p : CaracaraProgram) : CaracaraProgram :=
+  match f with
+  | [] => p
+  | (mp, cls) :: rest =>
+      let new_rule := Seq (SeqCtr mp [StatefulOp AddOp (ConstantArg (CrUInt8 cls)) (ConstantArg (CrUInt8 (repr 0))) (StateCtr 1)]) in
+      let t := get_transformer_from_prog p in
+      let new_transformer := new_rule :: t in
+      let new_prog := CaracaraProgramDef [] [] [] new_transformer in
+      db_to_simple_helper rest new_prog
+  end.
+Definition db_to_simple_classifier (f : FilterDatabase) : CaracaraProgram :=
+  let prog := db_to_simple_helper f (CaracaraProgramDef [] [] [] []) in
+  let t := get_transformer_from_prog prog in
+  let t' := List.rev t in
+  CaracaraProgramDef [] [] [] t'.
+
+Definition pkt_does_match (mp : MatchPattern) (pkt_h : PacketHeader) : bool :=
+  List.forallb (fun '(h, v) =>
+    CrVal.eqb (pkt_h !! (get_key h)) (IntVal v)) mp.
+Definition run_filter_db (f : FilterDatabase) (pkt_h : PacketHeader) : option Class :=
+  match List.find (fun '(mp, _) => pkt_does_match mp pkt_h) f with
+  | Some (_, cls) => Some cls
+  | None => None
+  end.
+
+Definition db_classifier : Classifier := run_filter_db.
+
+(* A program, p, is a packet classifier under an interpretation, i, if
+ *   when a packet with a given header is processed by p,
+ *   the interpretation of the resulting state is the same as
+ *   the class assigned by running that filter db on said packet header.
+ *)
+Definition is_classifier
+  (p : CaracaraProgram)
+  (i : Interpretation)
+  (f : FilterDatabase) : Prop :=
+  forall (pkt_h : PacketHeader) (ps : ConcreteState),
+    (header_map ps) = pkt_h ->
+    i (eval_cr_program_concrete p ps) = run_filter_db f pkt_h.
+
+Definition simple_interpreter (ps : ConcreteState) : option Class :=
+  match (state_map ps) !! 1 with
+  | IntVal n => match n with
+    | CrUInt8 cls => Some cls
+    | _ => None
+    end
+  | _ => None
+  end.
+
+Theorem db_to_simple_classifier_correct :
+  forall (f : FilterDatabase),
+    is_classifier (db_to_simple_classifier f) simple_interpreter f.
+Proof.
+Admitted.
